formal/fstar/ocaml-output/RML_Eval.ml
@@ -69,23 +69,22 @@ let is_frac_or_exp_marker (c : FStar_Char.char) : Prims.bool=
   let i = FStar_Char.int_of_char c in
   ((i = (Prims.of_int (0x2E))) || (i = (Prims.of_int (0x65)))) ||
     (i = (Prims.of_int (0x45)))
-let json_number_natural_datatype (lex : Prims.string) :
-  RDF_Graph_Executable.wf_iri=
+let json_number_natural_datatype (lex : Prims.string) : RDF_Term.wf_iri=
   if
     FStar_List_Tot_Base.existsb is_frac_or_exp_marker
       (FStar_String.list_of_string lex)
-  then RDF_Graph_Executable.xsd_double
-  else RDF_Graph_Executable.xsd_integer
+  then RDF_Term.xsd_double
+  else RDF_Term.xsd_integer
 let json_natural_value (v : Parser_JSON.json_val) :
-  (Prims.string * RDF_Graph_Executable.wf_iri) FStar_Pervasives_Native.option=
+  (Prims.string * RDF_Term.wf_iri) FStar_Pervasives_Native.option=
   match v with
   | Parser_JSON.JString s ->
-      FStar_Pervasives_Native.Some (s, RDF_Graph_Executable.xsd_string)
+      FStar_Pervasives_Native.Some (s, RDF_Term.xsd_string)
   | Parser_JSON.JNumber s ->
       FStar_Pervasives_Native.Some (s, (json_number_natural_datatype s))
   | Parser_JSON.JBool b ->
       FStar_Pervasives_Native.Some
-        ((if b then "true" else "false"), RDF_Graph_Executable.xsd_boolean)
+        ((if b then "true" else "false"), RDF_Term.xsd_boolean)
   | Parser_JSON.JNull -> FStar_Pervasives_Native.None
   | Parser_JSON.JArray uu___ -> FStar_Pervasives_Native.None
   | Parser_JSON.JObject uu___ -> FStar_Pervasives_Native.None
@@ -95,8 +94,7 @@ let json_natural_cast_string (v : Parser_JSON.json_val) :
   | FStar_Pervasives_Native.Some (s, uu___) -> FStar_Pervasives_Native.Some s
   | FStar_Pervasives_Native.None -> FStar_Pervasives_Native.None
 let reference_natural_values (row : RML_Sources.source_row)
-  (path : Prims.string) :
-  (Prims.string * RDF_Graph_Executable.wf_iri) Prims.list=
+  (path : Prims.string) : (Prims.string * RDF_Term.wf_iri) Prims.list=
   match row with
   | RML_Sources.Row_JSON uu___ ->
       FStar_List_Tot_Base.concatMap
@@ -106,7 +104,7 @@ let reference_natural_values (row : RML_Sources.source_row)
            | FStar_Pervasives_Native.None -> [])
         (RML_Sources.json_reference_values row path)
   | RML_Sources.Row_CSV uu___ ->
-      FStar_List_Tot_Base.map (fun v -> (v, RDF_Graph_Executable.xsd_string))
+      FStar_List_Tot_Base.map (fun v -> (v, RDF_Term.xsd_string))
         (RML_Sources.csv_reference_values row path)
 let reference_cast_strings (row : RML_Sources.source_row)
   (path : Prims.string) : Prims.string Prims.list=
@@ -196,57 +194,53 @@ let rec rml_iri_scan_wf (s : Prims.string) (pos : Prims.nat)
        then false
        else rml_iri_scan_wf s (pos + Prims.int_one) (fuel - Prims.int_one))
 let rml_is_valid_absolute_iri (s : Prims.string) : Prims.bool=
-  (RDF_Graph_Executable.is_iri s) &&
+  (RDF_Term.is_iri s) &&
     (rml_iri_scan_wf s Prims.int_zero
        ((FStar_String.strlen s) + Prims.int_one))
 let iri_like_term_gated (strict : Prims.bool) (value : Prims.string)
   (base_iri : Prims.string FStar_Pervasives_Native.option) :
-  RDF_Graph_Executable.rdf_term FStar_Pervasives_Native.option=
+  RDF_Term.rdf_term FStar_Pervasives_Native.option=
   let ok s =
-    if strict
-    then rml_is_valid_absolute_iri s
-    else RDF_Graph_Executable.is_iri s in
+    if strict then rml_is_valid_absolute_iri s else RDF_Term.is_iri s in
   if ok value
-  then FStar_Pervasives_Native.Some (RDF_Graph_Executable.T_IRI value)
+  then FStar_Pervasives_Native.Some (RDF_Term.T_IRI value)
   else
     (match base_iri with
      | FStar_Pervasives_Native.Some b ->
          let combined = Prims.strcat b value in
          if ok combined
-         then
-           FStar_Pervasives_Native.Some (RDF_Graph_Executable.T_IRI combined)
+         then FStar_Pervasives_Native.Some (RDF_Term.T_IRI combined)
          else FStar_Pervasives_Native.None
      | FStar_Pervasives_Native.None -> FStar_Pervasives_Native.None)
 let iri_like_term (value : Prims.string)
   (base_iri : Prims.string FStar_Pervasives_Native.option) :
-  RDF_Graph_Executable.rdf_term FStar_Pervasives_Native.option=
+  RDF_Term.rdf_term FStar_Pervasives_Native.option=
   iri_like_term_gated true value base_iri
 let eval_plain_strings (tm : RML_Mapping.term_map)
   (row : RML_Sources.source_row) : Prims.string Prims.list=
   match tm.RML_Mapping.tmap_form with
   | RML_Mapping.TMF_Constant t ->
       (match t with
-       | RDF_Graph_Executable.T_IRI i -> [i]
-       | RDF_Graph_Executable.T_Literal l ->
-           [l.RDF_Graph_Executable.lexical_form]
-       | RDF_Graph_Executable.T_BNode uu___ -> [])
+       | RDF_Term.T_IRI i -> [i]
+       | RDF_Term.T_Literal l -> [l.RDF_Term.lexical_form]
+       | RDF_Term.T_BNode uu___ -> [])
   | RML_Mapping.TMF_Reference r -> reference_cast_strings row r
   | RML_Mapping.TMF_Template t ->
       eval_template_strings FStar_Pervasives_Native.None t row
   | RML_Mapping.TMF_Unknown -> []
 let build_literal_opt (lex : Prims.string) (dt : Prims.string)
   (lang : Prims.string FStar_Pervasives_Native.option) :
-  RDF_Graph_Executable.rdf_term FStar_Pervasives_Native.option=
-  if RDF_Graph_Executable.is_iri dt
+  RDF_Term.rdf_term FStar_Pervasives_Native.option=
+  if RDF_Term.is_iri dt
   then
     let l =
       {
-        RDF_Graph_Executable.lexical_form = lex;
-        RDF_Graph_Executable.datatype = dt;
-        RDF_Graph_Executable.lang_tag = lang
+        RDF_Term.lexical_form = lex;
+        RDF_Term.datatype = dt;
+        RDF_Term.lang_tag = lang
       } in
-    (if RDF_Graph_Executable.literal_wf l
-     then FStar_Pervasives_Native.Some (RDF_Graph_Executable.T_Literal l)
+    (if RDF_Term.literal_wf l
+     then FStar_Pervasives_Native.Some (RDF_Term.T_Literal l)
      else FStar_Pervasives_Native.None)
   else FStar_Pervasives_Native.None
 let eval_iri_valued_strings (tm : RML_Mapping.term_map)
@@ -255,11 +249,11 @@ let eval_iri_valued_strings (tm : RML_Mapping.term_map)
   Prims.string Prims.list=
   let resolve s =
     match iri_like_term s base_iri with
-    | FStar_Pervasives_Native.Some (RDF_Graph_Executable.T_IRI i) -> [i]
+    | FStar_Pervasives_Native.Some (RDF_Term.T_IRI i) -> [i]
     | uu___ -> [] in
   match tm.RML_Mapping.tmap_form with
   | RML_Mapping.TMF_Constant t ->
-      (match t with | RDF_Graph_Executable.T_IRI i -> [i] | uu___ -> [])
+      (match t with | RDF_Term.T_IRI i -> [i] | uu___ -> [])
   | RML_Mapping.TMF_Reference r ->
       FStar_List_Tot_Base.concatMap resolve (reference_cast_strings row r)
   | RML_Mapping.TMF_Template t ->
@@ -308,15 +302,15 @@ let rml_lang_tag_wf (s : Prims.string) : Prims.bool=
 let literal_terms_for_base (tm : RML_Mapping.term_map)
   (row : RML_Sources.source_row)
   (base_iri : Prims.string FStar_Pervasives_Native.option)
-  (natural_dt : RDF_Graph_Executable.wf_iri) (lex : Prims.string) :
-  RDF_Graph_Executable.rdf_term Prims.list=
+  (natural_dt : RDF_Term.wf_iri) (lex : Prims.string) :
+  RDF_Term.rdf_term Prims.list=
   match tm.RML_Mapping.tmap_language with
   | FStar_Pervasives_Native.Some lang_tm ->
       FStar_List_Tot_Base.concatMap
         (fun lang ->
            if rml_lang_tag_wf lang
            then
-             match build_literal_opt lex RDF_Graph_Executable.rdf_lang_string
+             match build_literal_opt lex RDF_Term.rdf_lang_string
                      (FStar_Pervasives_Native.Some lang)
              with
              | FStar_Pervasives_Native.Some t -> [t]
@@ -339,28 +333,27 @@ let literal_terms_for_base (tm : RML_Mapping.term_map)
             | FStar_Pervasives_Native.Some t -> [t]
             | FStar_Pervasives_Native.None -> []))
 type resolved_value =
-  | RV_Value of Prims.string * RDF_Graph_Executable.wf_iri 
+  | RV_Value of Prims.string * RDF_Term.wf_iri 
   | RV_String of Prims.string 
 let uu___is_RV_Value (projectee : resolved_value) : Prims.bool=
   match projectee with | RV_Value (_0, _1) -> true | uu___ -> false
 let __proj__RV_Value__item___0 (projectee : resolved_value) : Prims.string=
   match projectee with | RV_Value (_0, _1) -> _0
 let __proj__RV_Value__item___1 (projectee : resolved_value) :
-  RDF_Graph_Executable.wf_iri= match projectee with | RV_Value (_0, _1) -> _1
+  RDF_Term.wf_iri= match projectee with | RV_Value (_0, _1) -> _1
 let uu___is_RV_String (projectee : resolved_value) : Prims.bool=
   match projectee with | RV_String _0 -> true | uu___ -> false
 let __proj__RV_String__item___0 (projectee : resolved_value) : Prims.string=
   match projectee with | RV_String _0 -> _0
 let resolved_value_natural (rv : resolved_value) :
-  (Prims.string * RDF_Graph_Executable.wf_iri) FStar_Pervasives_Native.option=
+  (Prims.string * RDF_Term.wf_iri) FStar_Pervasives_Native.option=
   match rv with
   | RV_Value (s, dt) -> FStar_Pervasives_Native.Some (s, dt)
-  | RV_String s ->
-      FStar_Pervasives_Native.Some (s, RDF_Graph_Executable.xsd_string)
+  | RV_String s -> FStar_Pervasives_Native.Some (s, RDF_Term.xsd_string)
 let finalize_value (tt : RML_Mapping.term_type) (tm : RML_Mapping.term_map)
   (row : RML_Sources.source_row)
   (base_iri : Prims.string FStar_Pervasives_Native.option)
-  (rv : resolved_value) : RDF_Graph_Executable.rdf_term Prims.list=
+  (rv : resolved_value) : RDF_Term.rdf_term Prims.list=
   match resolved_value_natural rv with
   | FStar_Pervasives_Native.None -> []
   | FStar_Pervasives_Native.Some (s, dt) ->
@@ -377,23 +370,23 @@ let finalize_value (tt : RML_Mapping.term_type) (tm : RML_Mapping.term_map)
            (match iri_like_term_gated false s base_iri with
             | FStar_Pervasives_Native.Some t -> [t]
             | FStar_Pervasives_Native.None -> [])
-       | RML_Mapping.TT_BlankNode -> [RDF_Graph_Executable.T_BNode s]
+       | RML_Mapping.TT_BlankNode -> [RDF_Term.T_BNode s]
        | RML_Mapping.TT_Literal ->
            literal_terms_for_base tm row base_iri dt s)
 let eval_term_map (role : map_role) (tm : RML_Mapping.term_map)
   (row : RML_Sources.source_row) (row_seed : Prims.string)
   (base_iri : Prims.string FStar_Pervasives_Native.option) :
-  RDF_Graph_Executable.rdf_term Prims.list=
+  RDF_Term.rdf_term Prims.list=
   match tm.RML_Mapping.tmap_form with
   | RML_Mapping.TMF_Constant t ->
       (match t with
-       | RDF_Graph_Executable.T_IRI uu___ -> [t]
-       | RDF_Graph_Executable.T_Literal uu___ -> [t]
-       | RDF_Graph_Executable.T_BNode uu___ -> [])
+       | RDF_Term.T_IRI uu___ -> [t]
+       | RDF_Term.T_Literal uu___ -> [t]
+       | RDF_Term.T_BNode uu___ -> [])
   | RML_Mapping.TMF_Unknown ->
       (match tm.RML_Mapping.tmap_termtype with
        | FStar_Pervasives_Native.Some (RML_Mapping.TT_BlankNode) ->
-           [RDF_Graph_Executable.T_BNode row_seed]
+           [RDF_Term.T_BNode row_seed]
        | uu___ -> [])
   | RML_Mapping.TMF_Reference r ->
       let tt = effective_term_type role tm in
@@ -415,23 +408,190 @@ let eval_term_map (role : map_role) (tm : RML_Mapping.term_map)
       let strs = eval_template_strings encode t row in
       FStar_List_Tot_Base.concatMap
         (fun s -> finalize_value tt tm row base_iri (RV_String s)) strs
+let rdf_nil_iri : RDF_Term.wf_iri=
+  "http://www.w3.org/1999/02/22-rdf-syntax-ns#nil"
+let rdf_Bag_iri : RDF_Term.wf_iri=
+  "http://www.w3.org/1999/02/22-rdf-syntax-ns#Bag"
+let rdf_Seq_iri : RDF_Term.wf_iri=
+  "http://www.w3.org/1999/02/22-rdf-syntax-ns#Seq"
+let rdf_Alt_iri : RDF_Term.wf_iri=
+  "http://www.w3.org/1999/02/22-rdf-syntax-ns#Alt"
+let rdf_type_iri : RDF_Term.wf_iri=
+  "http://www.w3.org/1999/02/22-rdf-syntax-ns#type"
+let mk_wf_iri (s : Prims.string) :
+  RDF_Term.wf_iri FStar_Pervasives_Native.option=
+  if RDF_Term.is_iri s
+  then FStar_Pervasives_Native.Some s
+  else FStar_Pervasives_Native.None
+let rdf_member_pred (i : Prims.nat) :
+  RDF_Term.wf_iri FStar_Pervasives_Native.option=
+  mk_wf_iri
+    (Prims.strcat "http://www.w3.org/1999/02/22-rdf-syntax-ns#_"
+       (Prims.string_of_int i))
+let gather_member_values (gm : RML_Mapping.gather_map)
+  (row : RML_Sources.source_row) (seed : Prims.string)
+  (base : Prims.string FStar_Pervasives_Native.option) :
+  RDF_Term.rdf_term Prims.list=
+  FStar_List_Tot_Base.concatMap
+    (fun tm -> eval_term_map MR_Object tm row seed base)
+    gm.RML_Mapping.gm_members
+let gather_heads (gm : RML_Mapping.gather_map) (row : RML_Sources.source_row)
+  (seed : Prims.string) (base : Prims.string FStar_Pervasives_Native.option)
+  : RDF_Term.subject Prims.list=
+  match (gm.RML_Mapping.gm_head).RML_Mapping.tmap_form with
+  | RML_Mapping.TMF_Unknown -> [RDF_Term.S_BNode (Prims.strcat seed "h")]
+  | uu___ ->
+      FStar_List_Tot_Base.concatMap
+        (fun t ->
+           match t with
+           | RDF_Term.T_IRI i -> [RDF_Term.S_IRI i]
+           | RDF_Term.T_BNode b -> [RDF_Term.S_BNode b]
+           | RDF_Term.T_Literal uu___1 -> [])
+        (eval_term_map MR_Object gm.RML_Mapping.gm_head row seed base)
+let rec build_list_struct (headsubj : RDF_Term.subject)
+  (members : RDF_Term.rdf_term Prims.list) (seed : Prims.string)
+  (k : Prims.nat) : RDF_Triple.triple Prims.list=
+  match members with
+  | [] -> []
+  | m::[] ->
+      [{
+         RDF_Triple.s = headsubj;
+         RDF_Triple.p = RML_Mapping.rdf_first_iri;
+         RDF_Triple.o = m
+       };
+      {
+        RDF_Triple.s = headsubj;
+        RDF_Triple.p = RML_Mapping.rdf_rest_iri;
+        RDF_Triple.o = (RDF_Term.T_IRI rdf_nil_iri)
+      }]
+  | m::rest ->
+      let next =
+        RDF_Term.S_BNode
+          (Prims.strcat seed (Prims.strcat "c" (Prims.string_of_int k))) in
+      {
+        RDF_Triple.s = headsubj;
+        RDF_Triple.p = RML_Mapping.rdf_first_iri;
+        RDF_Triple.o = m
+      } ::
+        {
+          RDF_Triple.s = headsubj;
+          RDF_Triple.p = RML_Mapping.rdf_rest_iri;
+          RDF_Triple.o = (SPARQL11_Algebra.subject_to_term next)
+        } :: (build_list_struct next rest seed (k + Prims.int_one))
+let rec build_container_members (headsubj : RDF_Term.subject)
+  (members : RDF_Term.rdf_term Prims.list) (i : Prims.nat) :
+  RDF_Triple.triple Prims.list=
+  match members with
+  | [] -> []
+  | m::rest ->
+      (match rdf_member_pred i with
+       | FStar_Pervasives_Native.Some p ->
+           { RDF_Triple.s = headsubj; RDF_Triple.p = p; RDF_Triple.o = m } ::
+           (build_container_members headsubj rest (i + Prims.int_one))
+       | FStar_Pervasives_Native.None ->
+           build_container_members headsubj rest (i + Prims.int_one))
+let collection_triples (kind : RML_Mapping.gather_as)
+  (allow_empty : Prims.bool) (headsubj : RDF_Term.subject)
+  (members : RDF_Term.rdf_term Prims.list) (seed : Prims.string) :
+  (RDF_Term.rdf_term FStar_Pervasives_Native.option * RDF_Triple.triple
+    Prims.list)=
+  match kind with
+  | RML_Mapping.GA_List ->
+      (match members with
+       | [] ->
+           if allow_empty
+           then
+             ((FStar_Pervasives_Native.Some (RDF_Term.T_IRI rdf_nil_iri)),
+               [])
+           else (FStar_Pervasives_Native.None, [])
+       | uu___ ->
+           ((FStar_Pervasives_Native.Some
+               (SPARQL11_Algebra.subject_to_term headsubj)),
+             (build_list_struct headsubj members seed Prims.int_one)))
+  | RML_Mapping.GA_Bag ->
+      let tyiri =
+        match kind with
+        | RML_Mapping.GA_Bag -> rdf_Bag_iri
+        | RML_Mapping.GA_Seq -> rdf_Seq_iri
+        | uu___ -> rdf_Alt_iri in
+      let type_t =
+        {
+          RDF_Triple.s = headsubj;
+          RDF_Triple.p = rdf_type_iri;
+          RDF_Triple.o = (RDF_Term.T_IRI tyiri)
+        } in
+      (match members with
+       | [] ->
+           if allow_empty
+           then
+             ((FStar_Pervasives_Native.Some
+                 (SPARQL11_Algebra.subject_to_term headsubj)), [type_t])
+           else (FStar_Pervasives_Native.None, [])
+       | uu___ ->
+           ((FStar_Pervasives_Native.Some
+               (SPARQL11_Algebra.subject_to_term headsubj)), (type_t ::
+             (build_container_members headsubj members Prims.int_one))))
+  | RML_Mapping.GA_Seq ->
+      let tyiri =
+        match kind with
+        | RML_Mapping.GA_Bag -> rdf_Bag_iri
+        | RML_Mapping.GA_Seq -> rdf_Seq_iri
+        | uu___ -> rdf_Alt_iri in
+      let type_t =
+        {
+          RDF_Triple.s = headsubj;
+          RDF_Triple.p = rdf_type_iri;
+          RDF_Triple.o = (RDF_Term.T_IRI tyiri)
+        } in
+      (match members with
+       | [] ->
+           if allow_empty
+           then
+             ((FStar_Pervasives_Native.Some
+                 (SPARQL11_Algebra.subject_to_term headsubj)), [type_t])
+           else (FStar_Pervasives_Native.None, [])
+       | uu___ ->
+           ((FStar_Pervasives_Native.Some
+               (SPARQL11_Algebra.subject_to_term headsubj)), (type_t ::
+             (build_container_members headsubj members Prims.int_one))))
+  | RML_Mapping.GA_Alt ->
+      let tyiri =
+        match kind with
+        | RML_Mapping.GA_Bag -> rdf_Bag_iri
+        | RML_Mapping.GA_Seq -> rdf_Seq_iri
+        | uu___ -> rdf_Alt_iri in
+      let type_t =
+        {
+          RDF_Triple.s = headsubj;
+          RDF_Triple.p = rdf_type_iri;
+          RDF_Triple.o = (RDF_Term.T_IRI tyiri)
+        } in
+      (match members with
+       | [] ->
+           if allow_empty
+           then
+             ((FStar_Pervasives_Native.Some
+                 (SPARQL11_Algebra.subject_to_term headsubj)), [type_t])
+           else (FStar_Pervasives_Native.None, [])
+       | uu___ ->
+           ((FStar_Pervasives_Native.Some
+               (SPARQL11_Algebra.subject_to_term headsubj)), (type_t ::
+             (build_container_members headsubj members Prims.int_one))))
+  | RML_Mapping.GA_Other uu___ -> (FStar_Pervasives_Native.None, [])
 let list_nonempty (l : 'a Prims.list) : Prims.bool=
   match l with | [] -> false | uu___ -> true
-let subject_of_rdf_term (t : RDF_Graph_Executable.rdf_term) :
-  RDF_Graph_Executable.subject FStar_Pervasives_Native.option=
+let subject_of_rdf_term (t : RDF_Term.rdf_term) :
+  RDF_Term.subject FStar_Pervasives_Native.option=
   match t with
-  | RDF_Graph_Executable.T_IRI i ->
-      FStar_Pervasives_Native.Some (RDF_Graph_Executable.S_IRI i)
-  | RDF_Graph_Executable.T_BNode b ->
-      FStar_Pervasives_Native.Some (RDF_Graph_Executable.S_BNode b)
-  | RDF_Graph_Executable.T_Literal uu___ -> FStar_Pervasives_Native.None
-let term_to_graph_name (t : RDF_Graph_Executable.rdf_term) :
+  | RDF_Term.T_IRI i -> FStar_Pervasives_Native.Some (RDF_Term.S_IRI i)
+  | RDF_Term.T_BNode b -> FStar_Pervasives_Native.Some (RDF_Term.S_BNode b)
+  | RDF_Term.T_Literal uu___ -> FStar_Pervasives_Native.None
+let term_to_graph_name (t : RDF_Term.rdf_term) :
   Prims.string FStar_Pervasives_Native.option=
   match t with
-  | RDF_Graph_Executable.T_IRI i -> FStar_Pervasives_Native.Some i
-  | RDF_Graph_Executable.T_BNode b ->
-      FStar_Pervasives_Native.Some (Prims.strcat "_:" b)
-  | RDF_Graph_Executable.T_Literal uu___ -> FStar_Pervasives_Native.None
+  | RDF_Term.T_IRI i -> FStar_Pervasives_Native.Some i
+  | RDF_Term.T_BNode b -> FStar_Pervasives_Native.Some (Prims.strcat "_:" b)
+  | RDF_Term.T_Literal uu___ -> FStar_Pervasives_Native.None
 let eval_graphs (gms : RML_Mapping.term_map Prims.list)
   (row : RML_Sources.source_row) (row_seed : Prims.string)
   (base_iri : Prims.string FStar_Pervasives_Native.option) :
@@ -446,11 +606,11 @@ let eval_graphs (gms : RML_Mapping.term_map Prims.list)
          (eval_term_map MR_Graph g row row_seed base_iri)) gms
 type placed_triple =
   {
-  pt_triple: RDF_Graph_Executable.triple ;
+  pt_triple: RDF_Triple.triple ;
   pt_graphs: Prims.string Prims.list ;
   pt_drop: Prims.bool }
 let __proj__Mkplaced_triple__item__pt_triple (projectee : placed_triple) :
-  RDF_Graph_Executable.triple=
+  RDF_Triple.triple=
   match projectee with | { pt_triple; pt_graphs; pt_drop;_} -> pt_triple
 let __proj__Mkplaced_triple__item__pt_graphs (projectee : placed_triple) :
   Prims.string Prims.list=
@@ -461,8 +621,8 @@ let __proj__Mkplaced_triple__item__pt_drop (projectee : placed_triple) :
 let eval_pom (row : RML_Sources.source_row) (row_seed : Prims.string)
   (base_iri : Prims.string FStar_Pervasives_Native.option)
   (pom : RML_Mapping.predicate_object_map) :
-  (RDF_Graph_Executable.rdf_term Prims.list * RDF_Graph_Executable.rdf_term
-    Prims.list * Prims.string Prims.list)=
+  (RDF_Term.rdf_term Prims.list * RDF_Term.rdf_term Prims.list * Prims.string
+    Prims.list)=
   let predicates =
     FStar_List_Tot_Base.concatMap
       (fun p -> eval_term_map MR_Predicate p row row_seed base_iri)
@@ -473,10 +633,59 @@ let eval_pom (row : RML_Sources.source_row) (row_seed : Prims.string)
          match ob with
          | RML_Mapping.OB_TermMap tm ->
              eval_term_map MR_Object tm row row_seed base_iri
-         | RML_Mapping.OB_Join uu___ -> []) pom.RML_Mapping.pom_objects in
+         | RML_Mapping.OB_Join uu___ -> []
+         | RML_Mapping.OB_Gather uu___ -> []) pom.RML_Mapping.pom_objects in
   let graphs = eval_graphs pom.RML_Mapping.pom_graphs row row_seed base_iri in
   (predicates, objects, graphs)
-let placed_triples_for_pom (subj : RDF_Graph_Executable.subject)
+let gather_placed_triples (subj : RDF_Term.subject)
+  (target : Prims.string Prims.list) (drop : Prims.bool)
+  (predicates : RDF_Term.rdf_term Prims.list) (gm : RML_Mapping.gather_map)
+  (row : RML_Sources.source_row) (seed : Prims.string)
+  (base : Prims.string FStar_Pervasives_Native.option) :
+  placed_triple Prims.list=
+  let members = gather_member_values gm row seed base in
+  let heads = gather_heads gm row seed base in
+  FStar_List_Tot_Base.concatMap
+    (fun uu___ ->
+       match uu___ with
+       | (hidx, headsubj) ->
+           let uu___1 =
+             collection_triples gm.RML_Mapping.gm_as
+               gm.RML_Mapping.gm_allow_empty headsubj members
+               (Prims.strcat seed
+                  (Prims.strcat "_" (Prims.string_of_int hidx))) in
+           (match uu___1 with
+            | (obj_opt, struct_ts) ->
+                (match obj_opt with
+                 | FStar_Pervasives_Native.None -> []
+                 | FStar_Pervasives_Native.Some obj ->
+                     let link_pts =
+                       FStar_List_Tot_Base.concatMap
+                         (fun p ->
+                            match p with
+                            | RDF_Term.T_IRI pi ->
+                                [{
+                                   pt_triple =
+                                     {
+                                       RDF_Triple.s = subj;
+                                       RDF_Triple.p = pi;
+                                       RDF_Triple.o = obj
+                                     };
+                                   pt_graphs = target;
+                                   pt_drop = drop
+                                 }]
+                            | uu___2 -> []) predicates in
+                     let struct_pts =
+                       FStar_List_Tot_Base.map
+                         (fun t ->
+                            {
+                              pt_triple = t;
+                              pt_graphs = target;
+                              pt_drop = drop
+                            }) struct_ts in
+                     FStar_List_Tot_Base.append link_pts struct_pts)))
+    (FStar_List_Tot_Base.mapi (fun i h -> (i, h)) heads)
+let placed_triples_for_pom (subj : RDF_Term.subject)
   (subject_graphs : Prims.string Prims.list) (has_sgm : Prims.bool)
   (row : RML_Sources.source_row) (row_seed : Prims.string)
   (base_iri : Prims.string FStar_Pervasives_Native.option)
@@ -490,27 +699,43 @@ let placed_triples_for_pom (subj : RDF_Graph_Executable.subject)
         then []
         else FStar_List_Tot_Base.op_At subject_graphs pog in
       let drop = (has_sgm || has_pogm) && (target = []) in
-      FStar_List_Tot_Base.concatMap
-        (fun p ->
-           match p with
-           | RDF_Graph_Executable.T_IRI pi ->
-               FStar_List_Tot_Base.concatMap
-                 (fun o ->
-                    [{
-                       pt_triple =
-                         {
-                           RDF_Graph_Executable.s = subj;
-                           RDF_Graph_Executable.p = pi;
-                           RDF_Graph_Executable.o = o
-                         };
-                       pt_graphs = target;
-                       pt_drop = drop
-                     }]) objects
-           | uu___1 -> []) predicates
-let class_placed_triples (subj : RDF_Graph_Executable.subject)
+      let plain_pts =
+        FStar_List_Tot_Base.concatMap
+          (fun p ->
+             match p with
+             | RDF_Term.T_IRI pi ->
+                 FStar_List_Tot_Base.concatMap
+                   (fun o ->
+                      [{
+                         pt_triple =
+                           {
+                             RDF_Triple.s = subj;
+                             RDF_Triple.p = pi;
+                             RDF_Triple.o = o
+                           };
+                         pt_graphs = target;
+                         pt_drop = drop
+                       }]) objects
+             | uu___1 -> []) predicates in
+      let gather_pts =
+        FStar_List_Tot_Base.concatMap
+          (fun uu___1 ->
+             match uu___1 with
+             | (gidx, ob) ->
+                 (match ob with
+                  | RML_Mapping.OB_Gather gm ->
+                      gather_placed_triples subj target drop predicates gm
+                        row
+                        (Prims.strcat row_seed
+                           (Prims.strcat "#g" (Prims.string_of_int gidx)))
+                        base_iri
+                  | uu___2 -> []))
+          (FStar_List_Tot_Base.mapi (fun i ob -> (i, ob))
+             pom.RML_Mapping.pom_objects) in
+      FStar_List_Tot_Base.append plain_pts gather_pts
+let class_placed_triples (subj : RDF_Term.subject)
   (subject_graphs : Prims.string Prims.list) (has_sgm : Prims.bool)
-  (classes : RDF_Graph_Executable.wf_iri Prims.list) :
-  placed_triple Prims.list=
+  (classes : RDF_Term.wf_iri Prims.list) : placed_triple Prims.list=
   let target = if has_sgm then subject_graphs else [] in
   let drop = has_sgm && (target = []) in
   FStar_List_Tot_Base.map
@@ -518,9 +743,9 @@ let class_placed_triples (subj : RDF_Graph_Executable.subject)
        {
          pt_triple =
            {
-             RDF_Graph_Executable.s = subj;
-             RDF_Graph_Executable.p = RDF_Graph_Executable.rdf_type;
-             RDF_Graph_Executable.o = (RDF_Graph_Executable.T_IRI cls)
+             RDF_Triple.s = subj;
+             RDF_Triple.p = RDFS_Closure.rdf_type;
+             RDF_Triple.o = (RDF_Term.T_IRI cls)
            };
          pt_graphs = target;
          pt_drop = drop
@@ -625,7 +850,7 @@ let matching_parent_rows (jcs : RML_Mapping.join_condition Prims.list)
            match uu___1 with
            | (uu___2, prow) -> join_conditions_hold jcs crow prow)
         parent_rows_idx
-let eval_join_pom (subj : RDF_Graph_Executable.subject)
+let eval_join_pom (subj : RDF_Term.subject)
   (subject_graphs : Prims.string Prims.list) (has_sgm : Prims.bool)
   (crow : RML_Sources.source_row) (cidx : Prims.int)
   (row_seed : Prims.string)
@@ -650,6 +875,7 @@ let eval_join_pom (subj : RDF_Graph_Executable.subject)
     (fun ob ->
        match ob with
        | RML_Mapping.OB_TermMap uu___ -> []
+       | RML_Mapping.OB_Gather uu___ -> []
        | RML_Mapping.OB_Join rom ->
            (match lookup_parent rom.RML_Mapping.rom_parent_triples_map with
             | FStar_Pervasives_Native.None -> []
@@ -680,16 +906,13 @@ let eval_join_pom (subj : RDF_Graph_Executable.subject)
                                    FStar_List_Tot_Base.concatMap
                                      (fun p ->
                                         match p with
-                                        | RDF_Graph_Executable.T_IRI pi ->
+                                        | RDF_Term.T_IRI pi ->
                                             [{
                                                pt_triple =
                                                  {
-                                                   RDF_Graph_Executable.s =
-                                                     subj;
-                                                   RDF_Graph_Executable.p =
-                                                     pi;
-                                                   RDF_Graph_Executable.o =
-                                                     obj_term
+                                                   RDF_Triple.s = subj;
+                                                   RDF_Triple.p = pi;
+                                                   RDF_Triple.o = obj_term
                                                  };
                                                pt_graphs = target;
                                                pt_drop = drop
@@ -735,53 +958,43 @@ let eval_join_triples_map (tmap : RML_Mapping.triples_map)
                           tmap.RML_Mapping.tm_predicate_object_maps)
                  subj_terms)
         (FStar_List_Tot_Base.mapi (fun i r -> (i, r)) rows)
-let add_to_named_graph (ds : RDF_Graph_Executable.rdf_dataset)
-  (name : Prims.string) (t : RDF_Graph_Executable.triple) :
-  RDF_Graph_Executable.rdf_dataset=
-  match FStar_List_Tot_Base.tryFind
-          (fun ng -> ng.RDF_Graph_Executable.ng_name = name)
-          ds.RDF_Graph_Executable.ds_named
+let add_to_named_graph (ds : RDF_Graph.rdf_dataset) (name : Prims.string)
+  (t : RDF_Triple.triple) : RDF_Graph.rdf_dataset=
+  match FStar_List_Tot_Base.tryFind (fun ng -> ng.RDF_Graph.ng_name = name)
+          ds.RDF_Graph.ds_named
   with
   | FStar_Pervasives_Native.Some uu___ ->
       {
-        RDF_Graph_Executable.ds_default =
-          (ds.RDF_Graph_Executable.ds_default);
-        RDF_Graph_Executable.ds_named =
+        RDF_Graph.ds_default = (ds.RDF_Graph.ds_default);
+        RDF_Graph.ds_named =
           (FStar_List_Tot_Base.map
              (fun ng ->
-                if ng.RDF_Graph_Executable.ng_name = name
+                if ng.RDF_Graph.ng_name = name
                 then
                   {
-                    RDF_Graph_Executable.ng_name =
-                      (ng.RDF_Graph_Executable.ng_name);
-                    RDF_Graph_Executable.ng_graph = (t ::
-                      (ng.RDF_Graph_Executable.ng_graph))
+                    RDF_Graph.ng_name = (ng.RDF_Graph.ng_name);
+                    RDF_Graph.ng_graph = (t :: (ng.RDF_Graph.ng_graph))
                   }
-                else ng) ds.RDF_Graph_Executable.ds_named)
+                else ng) ds.RDF_Graph.ds_named)
       }
   | FStar_Pervasives_Native.None ->
       {
-        RDF_Graph_Executable.ds_default =
-          (ds.RDF_Graph_Executable.ds_default);
-        RDF_Graph_Executable.ds_named =
-          ({
-             RDF_Graph_Executable.ng_name = name;
-             RDF_Graph_Executable.ng_graph = [t]
-           } :: (ds.RDF_Graph_Executable.ds_named))
+        RDF_Graph.ds_default = (ds.RDF_Graph.ds_default);
+        RDF_Graph.ds_named =
+          ({ RDF_Graph.ng_name = name; RDF_Graph.ng_graph = [t] } ::
+          (ds.RDF_Graph.ds_named))
       }
-let add_to_graph (ds : RDF_Graph_Executable.rdf_dataset)
-  (name : Prims.string) (t : RDF_Graph_Executable.triple) :
-  RDF_Graph_Executable.rdf_dataset=
+let add_to_graph (ds : RDF_Graph.rdf_dataset) (name : Prims.string)
+  (t : RDF_Triple.triple) : RDF_Graph.rdf_dataset=
   if name = RML_Mapping.rml_defaultGraph
   then
     {
-      RDF_Graph_Executable.ds_default = (t ::
-        (ds.RDF_Graph_Executable.ds_default));
-      RDF_Graph_Executable.ds_named = (ds.RDF_Graph_Executable.ds_named)
+      RDF_Graph.ds_default = (t :: (ds.RDF_Graph.ds_default));
+      RDF_Graph.ds_named = (ds.RDF_Graph.ds_named)
     }
   else add_to_named_graph ds name t
-let rec place_into_dataset (ds : RDF_Graph_Executable.rdf_dataset)
-  (pts : placed_triple Prims.list) : RDF_Graph_Executable.rdf_dataset=
+let rec place_into_dataset (ds : RDF_Graph.rdf_dataset)
+  (pts : placed_triple Prims.list) : RDF_Graph.rdf_dataset=
   match pts with
   | [] -> ds
   | pt::rest ->
@@ -792,10 +1005,9 @@ let rec place_into_dataset (ds : RDF_Graph_Executable.rdf_dataset)
           if pt.pt_graphs = []
           then
             {
-              RDF_Graph_Executable.ds_default = ((pt.pt_triple) ::
-                (ds.RDF_Graph_Executable.ds_default));
-              RDF_Graph_Executable.ds_named =
-                (ds.RDF_Graph_Executable.ds_named)
+              RDF_Graph.ds_default = ((pt.pt_triple) ::
+                (ds.RDF_Graph.ds_default));
+              RDF_Graph.ds_named = (ds.RDF_Graph.ds_named)
             }
           else
             FStar_List_Tot_Base.fold_left
@@ -808,24 +1020,24 @@ let eval_join_triples_map_dataset (tmap : RML_Mapping.triples_map)
     RML_Mapping.node_ref ->
       (RML_Mapping.triples_map * RML_Sources.source_row Prims.list)
         FStar_Pervasives_Native.option)
-  (ds : RDF_Graph_Executable.rdf_dataset) : RDF_Graph_Executable.rdf_dataset=
+  (ds : RDF_Graph.rdf_dataset) : RDF_Graph.rdf_dataset=
   place_into_dataset ds
     (eval_join_triples_map tmap rows default_base_iri lookup_parent)
 let eval_triples_map_dataset (tmap : RML_Mapping.triples_map)
   (rows : RML_Sources.source_row Prims.list)
   (default_base_iri : Prims.string FStar_Pervasives_Native.option) :
-  RDF_Graph_Executable.rdf_dataset=
-  place_into_dataset RDF_Graph_Executable.empty_dataset
+  RDF_Graph.rdf_dataset=
+  place_into_dataset RDF_Graph.empty_dataset
     (eval_triples_map tmap rows default_base_iri)
 let eval_triples_map_json_dataset (tmap : RML_Mapping.triples_map)
   (json_root : Parser_JSON.json_val)
   (default_base_iri : Prims.string FStar_Pervasives_Native.option) :
-  RDF_Graph_Executable.rdf_dataset=
-  place_into_dataset RDF_Graph_Executable.empty_dataset
+  RDF_Graph.rdf_dataset=
+  place_into_dataset RDF_Graph.empty_dataset
     (eval_triples_map_json tmap json_root default_base_iri)
 let eval_triples_map_csv_dataset (tmap : RML_Mapping.triples_map)
   (csv_text : Prims.string)
   (default_base_iri : Prims.string FStar_Pervasives_Native.option) :
-  RDF_Graph_Executable.rdf_dataset=
-  place_into_dataset RDF_Graph_Executable.empty_dataset
+  RDF_Graph.rdf_dataset=
+  place_into_dataset RDF_Graph.empty_dataset
     (eval_triples_map_csv tmap csv_text default_base_iri)
