formal/fstar/ocaml-output/RML_Mapping.ml
@@ -1,76 +1,72 @@
 open Prims
-let rml_TriplesMap : RDF_Graph_Executable.wf_iri=
-  "http://w3id.org/rml/TriplesMap"
-let rml_baseIRI : RDF_Graph_Executable.wf_iri= "http://w3id.org/rml/baseIRI"
-let rml_logicalSource : RDF_Graph_Executable.wf_iri=
-  "http://w3id.org/rml/logicalSource"
-let rml_iterator : RDF_Graph_Executable.wf_iri=
-  "http://w3id.org/rml/iterator"
-let rml_referenceFormulation : RDF_Graph_Executable.wf_iri=
+let rml_TriplesMap : RDF_Term.wf_iri= "http://w3id.org/rml/TriplesMap"
+let rml_baseIRI : RDF_Term.wf_iri= "http://w3id.org/rml/baseIRI"
+let rml_logicalSource : RDF_Term.wf_iri= "http://w3id.org/rml/logicalSource"
+let rml_iterator : RDF_Term.wf_iri= "http://w3id.org/rml/iterator"
+let rml_referenceFormulation : RDF_Term.wf_iri=
   "http://w3id.org/rml/referenceFormulation"
-let rml_JSONPath : RDF_Graph_Executable.wf_iri=
-  "http://w3id.org/rml/JSONPath"
-let rml_XPath : RDF_Graph_Executable.wf_iri= "http://w3id.org/rml/XPath"
-let rml_CSV : RDF_Graph_Executable.wf_iri= "http://w3id.org/rml/CSV"
-let rml_source : RDF_Graph_Executable.wf_iri= "http://w3id.org/rml/source"
-let rml_path : RDF_Graph_Executable.wf_iri= "http://w3id.org/rml/path"
-let rml_root : RDF_Graph_Executable.wf_iri= "http://w3id.org/rml/root"
-let rml_null : RDF_Graph_Executable.wf_iri= "http://w3id.org/rml/null"
-let rml_MappingDirectory : RDF_Graph_Executable.wf_iri=
+let rml_JSONPath : RDF_Term.wf_iri= "http://w3id.org/rml/JSONPath"
+let rml_XPath : RDF_Term.wf_iri= "http://w3id.org/rml/XPath"
+let rml_CSV : RDF_Term.wf_iri= "http://w3id.org/rml/CSV"
+let rml_source : RDF_Term.wf_iri= "http://w3id.org/rml/source"
+let rml_path : RDF_Term.wf_iri= "http://w3id.org/rml/path"
+let rml_root : RDF_Term.wf_iri= "http://w3id.org/rml/root"
+let rml_null : RDF_Term.wf_iri= "http://w3id.org/rml/null"
+let rml_MappingDirectory : RDF_Term.wf_iri=
   "http://w3id.org/rml/MappingDirectory"
-let rml_CurrentWorkingDirectory : RDF_Graph_Executable.wf_iri=
+let rml_CurrentWorkingDirectory : RDF_Term.wf_iri=
   "http://w3id.org/rml/CurrentWorkingDirectory"
-let rml_subjectMap : RDF_Graph_Executable.wf_iri=
-  "http://w3id.org/rml/subjectMap"
-let rml_subject : RDF_Graph_Executable.wf_iri= "http://w3id.org/rml/subject"
-let rml_class : RDF_Graph_Executable.wf_iri= "http://w3id.org/rml/class"
-let rml_graph : RDF_Graph_Executable.wf_iri= "http://w3id.org/rml/graph"
-let rml_graphMap : RDF_Graph_Executable.wf_iri=
-  "http://w3id.org/rml/graphMap"
-let rml_defaultGraph : RDF_Graph_Executable.wf_iri=
-  "http://w3id.org/rml/defaultGraph"
-let rml_predicateObjectMap : RDF_Graph_Executable.wf_iri=
+let rml_subjectMap : RDF_Term.wf_iri= "http://w3id.org/rml/subjectMap"
+let rml_subject : RDF_Term.wf_iri= "http://w3id.org/rml/subject"
+let rml_class : RDF_Term.wf_iri= "http://w3id.org/rml/class"
+let rml_graph : RDF_Term.wf_iri= "http://w3id.org/rml/graph"
+let rml_graphMap : RDF_Term.wf_iri= "http://w3id.org/rml/graphMap"
+let rml_defaultGraph : RDF_Term.wf_iri= "http://w3id.org/rml/defaultGraph"
+let rml_predicateObjectMap : RDF_Term.wf_iri=
   "http://w3id.org/rml/predicateObjectMap"
-let rml_predicate : RDF_Graph_Executable.wf_iri=
-  "http://w3id.org/rml/predicate"
-let rml_predicateMap : RDF_Graph_Executable.wf_iri=
-  "http://w3id.org/rml/predicateMap"
-let rml_object : RDF_Graph_Executable.wf_iri= "http://w3id.org/rml/object"
-let rml_objectMap : RDF_Graph_Executable.wf_iri=
-  "http://w3id.org/rml/objectMap"
-let rml_parentTriplesMap : RDF_Graph_Executable.wf_iri=
+let rml_predicate : RDF_Term.wf_iri= "http://w3id.org/rml/predicate"
+let rml_predicateMap : RDF_Term.wf_iri= "http://w3id.org/rml/predicateMap"
+let rml_object : RDF_Term.wf_iri= "http://w3id.org/rml/object"
+let rml_objectMap : RDF_Term.wf_iri= "http://w3id.org/rml/objectMap"
+let rml_parentTriplesMap : RDF_Term.wf_iri=
   "http://w3id.org/rml/parentTriplesMap"
-let rml_joinCondition : RDF_Graph_Executable.wf_iri=
-  "http://w3id.org/rml/joinCondition"
-let rml_child : RDF_Graph_Executable.wf_iri= "http://w3id.org/rml/child"
-let rml_parent : RDF_Graph_Executable.wf_iri= "http://w3id.org/rml/parent"
-let rml_childMap : RDF_Graph_Executable.wf_iri=
-  "http://w3id.org/rml/childMap"
-let rml_parentMap : RDF_Graph_Executable.wf_iri=
-  "http://w3id.org/rml/parentMap"
-let rml_constant : RDF_Graph_Executable.wf_iri=
-  "http://w3id.org/rml/constant"
-let rml_reference : RDF_Graph_Executable.wf_iri=
-  "http://w3id.org/rml/reference"
-let rml_template : RDF_Graph_Executable.wf_iri=
-  "http://w3id.org/rml/template"
-let rml_termType : RDF_Graph_Executable.wf_iri=
-  "http://w3id.org/rml/termType"
-let rml_IRI : RDF_Graph_Executable.wf_iri= "http://w3id.org/rml/IRI"
-let rml_URI : RDF_Graph_Executable.wf_iri= "http://w3id.org/rml/URI"
-let rml_UnsafeIRI : RDF_Graph_Executable.wf_iri=
-  "http://w3id.org/rml/UnsafeIRI"
-let rml_BlankNode : RDF_Graph_Executable.wf_iri=
-  "http://w3id.org/rml/BlankNode"
-let rml_Literal : RDF_Graph_Executable.wf_iri= "http://w3id.org/rml/Literal"
-let rml_datatype : RDF_Graph_Executable.wf_iri=
-  "http://w3id.org/rml/datatype"
-let rml_datatypeMap : RDF_Graph_Executable.wf_iri=
-  "http://w3id.org/rml/datatypeMap"
-let rml_language : RDF_Graph_Executable.wf_iri=
-  "http://w3id.org/rml/language"
-let rml_languageMap : RDF_Graph_Executable.wf_iri=
-  "http://w3id.org/rml/languageMap"
+let rml_joinCondition : RDF_Term.wf_iri= "http://w3id.org/rml/joinCondition"
+let rml_child : RDF_Term.wf_iri= "http://w3id.org/rml/child"
+let rml_parent : RDF_Term.wf_iri= "http://w3id.org/rml/parent"
+let rml_childMap : RDF_Term.wf_iri= "http://w3id.org/rml/childMap"
+let rml_parentMap : RDF_Term.wf_iri= "http://w3id.org/rml/parentMap"
+let rml_constant : RDF_Term.wf_iri= "http://w3id.org/rml/constant"
+let rml_reference : RDF_Term.wf_iri= "http://w3id.org/rml/reference"
+let rml_template : RDF_Term.wf_iri= "http://w3id.org/rml/template"
+let rml_termType : RDF_Term.wf_iri= "http://w3id.org/rml/termType"
+let rml_IRI : RDF_Term.wf_iri= "http://w3id.org/rml/IRI"
+let rml_URI : RDF_Term.wf_iri= "http://w3id.org/rml/URI"
+let rml_UnsafeIRI : RDF_Term.wf_iri= "http://w3id.org/rml/UnsafeIRI"
+let rml_BlankNode : RDF_Term.wf_iri= "http://w3id.org/rml/BlankNode"
+let rml_Literal : RDF_Term.wf_iri= "http://w3id.org/rml/Literal"
+let rml_datatype : RDF_Term.wf_iri= "http://w3id.org/rml/datatype"
+let rml_datatypeMap : RDF_Term.wf_iri= "http://w3id.org/rml/datatypeMap"
+let rml_language : RDF_Term.wf_iri= "http://w3id.org/rml/language"
+let rml_languageMap : RDF_Term.wf_iri= "http://w3id.org/rml/languageMap"
+let rml_gather : RDF_Term.wf_iri= "http://w3id.org/rml/gather"
+let rml_gatherAs : RDF_Term.wf_iri= "http://w3id.org/rml/gatherAs"
+let rml_strategy : RDF_Term.wf_iri= "http://w3id.org/rml/strategy"
+let rml_allowEmptyListAndContainer : RDF_Term.wf_iri=
+  "http://w3id.org/rml/allowEmptyListAndContainer"
+let rml_cartesianProduct : RDF_Term.wf_iri=
+  "http://w3id.org/rml/cartesianProduct"
+let rdf_first_iri : RDF_Term.wf_iri=
+  "http://www.w3.org/1999/02/22-rdf-syntax-ns#first"
+let rdf_rest_iri : RDF_Term.wf_iri=
+  "http://www.w3.org/1999/02/22-rdf-syntax-ns#rest"
+let rdf_List_str : Prims.string=
+  "http://www.w3.org/1999/02/22-rdf-syntax-ns#List"
+let rdf_Bag_str : Prims.string=
+  "http://www.w3.org/1999/02/22-rdf-syntax-ns#Bag"
+let rdf_Seq_str : Prims.string=
+  "http://www.w3.org/1999/02/22-rdf-syntax-ns#Seq"
+let rdf_Alt_str : Prims.string=
+  "http://www.w3.org/1999/02/22-rdf-syntax-ns#Alt"
 type template_segment =
   | TSeg_Literal of Prims.string 
   | TSeg_Reference of Prims.string 
@@ -170,10 +166,10 @@ let uu___is_Root_Other (projectee : source_root) : Prims.bool=
   match projectee with | Root_Other _0 -> true | uu___ -> false
 let __proj__Root_Other__item___0 (projectee : source_root) : Prims.string=
   match projectee with | Root_Other _0 -> _0
-let decode_term_type (t : RDF_Graph_Executable.rdf_term) :
+let decode_term_type (t : RDF_Term.rdf_term) :
   term_type FStar_Pervasives_Native.option=
   match t with
-  | RDF_Graph_Executable.T_IRI i ->
+  | RDF_Term.T_IRI i ->
       if i = rml_IRI
       then FStar_Pervasives_Native.Some TT_IRI
       else
@@ -190,10 +186,10 @@ let decode_term_type (t : RDF_Graph_Executable.rdf_term) :
               then FStar_Pervasives_Native.Some TT_Literal
               else FStar_Pervasives_Native.None
   | uu___ -> FStar_Pervasives_Native.None
-let decode_reference_formulation (t : RDF_Graph_Executable.rdf_term) :
+let decode_reference_formulation (t : RDF_Term.rdf_term) :
   reference_formulation=
   match t with
-  | RDF_Graph_Executable.T_IRI i ->
+  | RDF_Term.T_IRI i ->
       if i = rml_JSONPath
       then RF_JSONPath
       else
@@ -201,9 +197,9 @@ let decode_reference_formulation (t : RDF_Graph_Executable.rdf_term) :
         then RF_XPath
         else if i = rml_CSV then RF_CSV else RF_Other i
   | uu___ -> RF_Other ""
-let decode_source_root (t : RDF_Graph_Executable.rdf_term) : source_root=
+let decode_source_root (t : RDF_Term.rdf_term) : source_root=
   match t with
-  | RDF_Graph_Executable.T_IRI i ->
+  | RDF_Term.T_IRI i ->
       if i = rml_MappingDirectory
       then Root_MappingDirectory
       else
@@ -212,30 +208,26 @@ let decode_source_root (t : RDF_Graph_Executable.rdf_term) : source_root=
         else Root_Other i
   | uu___ -> Root_Other ""
 type node_ref = Prims.string
-let term_to_node_ref (t : RDF_Graph_Executable.rdf_term) :
+let term_to_node_ref (t : RDF_Term.rdf_term) :
   node_ref FStar_Pervasives_Native.option=
   match t with
-  | RDF_Graph_Executable.T_IRI i -> FStar_Pervasives_Native.Some i
-  | RDF_Graph_Executable.T_BNode b ->
-      FStar_Pervasives_Native.Some (Prims.strcat "_:" b)
-  | RDF_Graph_Executable.T_Literal uu___ -> FStar_Pervasives_Native.None
-let subject_to_node_ref (s : RDF_Graph_Executable.subject) : node_ref=
+  | RDF_Term.T_IRI i -> FStar_Pervasives_Native.Some i
+  | RDF_Term.T_BNode b -> FStar_Pervasives_Native.Some (Prims.strcat "_:" b)
+  | RDF_Term.T_Literal uu___ -> FStar_Pervasives_Native.None
+let subject_to_node_ref (s : RDF_Term.subject) : node_ref=
   match s with
-  | RDF_Graph_Executable.S_IRI i -> i
-  | RDF_Graph_Executable.S_BNode b -> Prims.strcat "_:" b
-let rec distinct_subjects_acc (g : RDF_Graph_Executable.rdf_graph)
-  (acc : RDF_Graph_Executable.subject Prims.list) :
-  RDF_Graph_Executable.subject Prims.list=
+  | RDF_Term.S_IRI i -> i
+  | RDF_Term.S_BNode b -> Prims.strcat "_:" b
+let rec distinct_subjects_acc (g : RDF_Graph.rdf_graph)
+  (acc : RDF_Term.subject Prims.list) : RDF_Term.subject Prims.list=
   match g with
   | [] -> acc
   | t::rest ->
-      if
-        FStar_List_Tot_Base.existsb
-          (RDF_Graph_Executable.subject_eq t.RDF_Graph_Executable.s) acc
+      if FStar_List_Tot_Base.existsb (RDF_Term.subject_eq t.RDF_Triple.s) acc
       then distinct_subjects_acc rest acc
-      else distinct_subjects_acc rest ((t.RDF_Graph_Executable.s) :: acc)
-let distinct_subjects (g : RDF_Graph_Executable.rdf_graph) :
-  RDF_Graph_Executable.subject Prims.list= distinct_subjects_acc g []
+      else distinct_subjects_acc rest ((t.RDF_Triple.s) :: acc)
+let distinct_subjects (g : RDF_Graph.rdf_graph) :
+  RDF_Term.subject Prims.list= distinct_subjects_acc g []
 type logical_source =
   {
   ls_iterator: Prims.string FStar_Pervasives_Native.option ;
@@ -278,27 +270,25 @@ let empty_logical_source : logical_source=
     ls_source_root = FStar_Pervasives_Native.None;
     ls_null_values = []
   }
-let first_literal (l : RDF_Graph_Executable.rdf_term Prims.list) :
+let first_literal (l : RDF_Term.rdf_term Prims.list) :
   Prims.string FStar_Pervasives_Native.option=
   match l with
-  | (RDF_Graph_Executable.T_Literal lit)::uu___ ->
-      FStar_Pervasives_Native.Some (lit.RDF_Graph_Executable.lexical_form)
+  | (RDF_Term.T_Literal lit)::uu___ ->
+      FStar_Pervasives_Native.Some (lit.RDF_Term.lexical_form)
   | uu___ -> FStar_Pervasives_Native.None
-let literal_strings (l : RDF_Graph_Executable.rdf_term Prims.list) :
+let literal_strings (l : RDF_Term.rdf_term Prims.list) :
   Prims.string Prims.list=
   FStar_List_Tot_Base.concatMap
     (fun t ->
        match t with
-       | RDF_Graph_Executable.T_Literal lit ->
-           [lit.RDF_Graph_Executable.lexical_form]
+       | RDF_Term.T_Literal lit -> [lit.RDF_Term.lexical_form]
        | uu___ -> []) l
-let decode_logical_source (g : RDF_Graph_Executable.rdf_graph)
-  (s : RDF_Graph_Executable.subject) :
+let decode_logical_source (g : RDF_Graph.rdf_graph) (s : RDF_Term.subject) :
   logical_source FStar_Pervasives_Native.option=
   match RDF_Graph_Executable.find_objects g s rml_logicalSource with
   | [] -> FStar_Pervasives_Native.None
   | ls_term::uu___ ->
-      (match RDF_Graph_Executable.term_to_subject ls_term with
+      (match RDF_Graph.term_to_subject ls_term with
        | FStar_Pervasives_Native.None -> FStar_Pervasives_Native.None
        | FStar_Pervasives_Native.Some ls_subj ->
            let iterator =
@@ -316,7 +306,7 @@ let decode_logical_source (g : RDF_Graph_Executable.rdf_graph)
              match RDF_Graph_Executable.find_objects g ls_subj rml_source
              with
              | src_term::uu___2 ->
-                 (match RDF_Graph_Executable.term_to_subject src_term with
+                 (match RDF_Graph.term_to_subject src_term with
                   | FStar_Pervasives_Native.Some src_subj ->
                       ((first_literal
                           (RDF_Graph_Executable.find_objects g src_subj
@@ -348,14 +338,14 @@ let decode_logical_source (g : RDF_Graph_Executable.rdf_graph)
                     ls_null_values = null_values
                   }))
 type term_map_form =
-  | TMF_Constant of RDF_Graph_Executable.rdf_term 
+  | TMF_Constant of RDF_Term.rdf_term 
   | TMF_Reference of Prims.string 
   | TMF_Template of Prims.string 
   | TMF_Unknown 
 let uu___is_TMF_Constant (projectee : term_map_form) : Prims.bool=
   match projectee with | TMF_Constant _0 -> true | uu___ -> false
 let __proj__TMF_Constant__item___0 (projectee : term_map_form) :
-  RDF_Graph_Executable.rdf_term= match projectee with | TMF_Constant _0 -> _0
+  RDF_Term.rdf_term= match projectee with | TMF_Constant _0 -> _0
 let uu___is_TMF_Reference (projectee : term_map_form) : Prims.bool=
   match projectee with | TMF_Reference _0 -> true | uu___ -> false
 let __proj__TMF_Reference__item___0 (projectee : term_map_form) :
@@ -398,7 +388,7 @@ let unknown_term_map : term_map=
     tmap_datatype = FStar_Pervasives_Native.None;
     tmap_language = FStar_Pervasives_Native.None
   }
-let const_term_map (t : RDF_Graph_Executable.rdf_term) : term_map=
+let const_term_map (t : RDF_Term.rdf_term) : term_map=
   {
     tmap_form = (TMF_Constant t);
     tmap_termtype = FStar_Pervasives_Native.None;
@@ -412,8 +402,8 @@ let ref_term_map (r : Prims.string) : term_map=
     tmap_datatype = FStar_Pervasives_Native.None;
     tmap_language = FStar_Pervasives_Native.None
   }
-let rec decode_term_map_from_subject (g : RDF_Graph_Executable.rdf_graph)
-  (s : RDF_Graph_Executable.subject) (fuel : Prims.nat) : term_map=
+let rec decode_term_map_from_subject (g : RDF_Graph.rdf_graph)
+  (s : RDF_Term.subject) (fuel : Prims.nat) : term_map=
   if fuel = Prims.int_zero
   then unknown_term_map
   else
@@ -423,13 +413,13 @@ let rec decode_term_map_from_subject (g : RDF_Graph_Executable.rdf_graph)
        | t::uu___1 -> TMF_Constant t
        | [] ->
            (match RDF_Graph_Executable.find_objects g s rml_reference with
-            | (RDF_Graph_Executable.T_Literal l)::uu___1 ->
-                TMF_Reference (l.RDF_Graph_Executable.lexical_form)
+            | (RDF_Term.T_Literal l)::uu___1 ->
+                TMF_Reference (l.RDF_Term.lexical_form)
             | uu___1 ->
                 (match RDF_Graph_Executable.find_objects g s rml_template
                  with
-                 | (RDF_Graph_Executable.T_Literal l)::uu___2 ->
-                     TMF_Template (l.RDF_Graph_Executable.lexical_form)
+                 | (RDF_Term.T_Literal l)::uu___2 ->
+                     TMF_Template (l.RDF_Term.lexical_form)
                  | uu___2 -> TMF_Unknown)) in
      let termtype =
        match RDF_Graph_Executable.find_objects g s rml_termType with
@@ -438,7 +428,7 @@ let rec decode_term_map_from_subject (g : RDF_Graph_Executable.rdf_graph)
      let datatype =
        match RDF_Graph_Executable.find_objects g s rml_datatypeMap with
        | t::uu___1 ->
-           (match RDF_Graph_Executable.term_to_subject t with
+           (match RDF_Graph.term_to_subject t with
             | FStar_Pervasives_Native.Some ds ->
                 FStar_Pervasives_Native.Some
                   (decode_term_map_from_subject g ds fuel')
@@ -450,7 +440,7 @@ let rec decode_term_map_from_subject (g : RDF_Graph_Executable.rdf_graph)
      let language =
        match RDF_Graph_Executable.find_objects g s rml_languageMap with
        | t::uu___1 ->
-           (match RDF_Graph_Executable.term_to_subject t with
+           (match RDF_Graph.term_to_subject t with
             | FStar_Pervasives_Native.Some ls ->
                 FStar_Pervasives_Native.Some
                   (decode_term_map_from_subject g ls fuel')
@@ -483,27 +473,25 @@ let __proj__Mkref_object_map__item__rom_parent_triples_map
 let __proj__Mkref_object_map__item__rom_joins (projectee : ref_object_map) :
   join_condition Prims.list=
   match projectee with | { rom_parent_triples_map; rom_joins;_} -> rom_joins
-let decode_child_or_parent (g : RDF_Graph_Executable.rdf_graph)
-  (s : RDF_Graph_Executable.subject) (map_pred : RDF_Graph_Executable.wf_iri)
-  (shortcut_pred : RDF_Graph_Executable.wf_iri) (fuel : Prims.nat) :
-  term_map=
+let decode_child_or_parent (g : RDF_Graph.rdf_graph) (s : RDF_Term.subject)
+  (map_pred : RDF_Term.wf_iri) (shortcut_pred : RDF_Term.wf_iri)
+  (fuel : Prims.nat) : term_map=
   match RDF_Graph_Executable.find_objects g s map_pred with
   | t::uu___ ->
-      (match RDF_Graph_Executable.term_to_subject t with
+      (match RDF_Graph.term_to_subject t with
        | FStar_Pervasives_Native.Some ms ->
            decode_term_map_from_subject g ms fuel
        | FStar_Pervasives_Native.None -> unknown_term_map)
   | [] ->
       (match RDF_Graph_Executable.find_objects g s shortcut_pred with
-       | (RDF_Graph_Executable.T_Literal l)::uu___ ->
-           ref_term_map l.RDF_Graph_Executable.lexical_form
+       | (RDF_Term.T_Literal l)::uu___ ->
+           ref_term_map l.RDF_Term.lexical_form
        | uu___ -> unknown_term_map)
-let decode_join_conditions (g : RDF_Graph_Executable.rdf_graph)
-  (s : RDF_Graph_Executable.subject) (fuel : Prims.nat) :
-  join_condition Prims.list=
+let decode_join_conditions (g : RDF_Graph.rdf_graph) (s : RDF_Term.subject)
+  (fuel : Prims.nat) : join_condition Prims.list=
   FStar_List_Tot_Base.concatMap
     (fun t ->
-       match RDF_Graph_Executable.term_to_subject t with
+       match RDF_Graph.term_to_subject t with
        | FStar_Pervasives_Native.None -> []
        | FStar_Pervasives_Native.Some jc_subj ->
            [{
@@ -513,9 +501,137 @@ let decode_join_conditions (g : RDF_Graph_Executable.rdf_graph)
                 (decode_child_or_parent g jc_subj rml_parentMap rml_parent
                    fuel)
             }]) (RDF_Graph_Executable.find_objects g s rml_joinCondition)
+type gather_as =
+  | GA_List 
+  | GA_Bag 
+  | GA_Seq 
+  | GA_Alt 
+  | GA_Other of Prims.string 
+let uu___is_GA_List (projectee : gather_as) : Prims.bool=
+  match projectee with | GA_List -> true | uu___ -> false
+let uu___is_GA_Bag (projectee : gather_as) : Prims.bool=
+  match projectee with | GA_Bag -> true | uu___ -> false
+let uu___is_GA_Seq (projectee : gather_as) : Prims.bool=
+  match projectee with | GA_Seq -> true | uu___ -> false
+let uu___is_GA_Alt (projectee : gather_as) : Prims.bool=
+  match projectee with | GA_Alt -> true | uu___ -> false
+let uu___is_GA_Other (projectee : gather_as) : Prims.bool=
+  match projectee with | GA_Other _0 -> true | uu___ -> false
+let __proj__GA_Other__item___0 (projectee : gather_as) : Prims.string=
+  match projectee with | GA_Other _0 -> _0
+type gather_strategy =
+  | GS_Append 
+  | GS_CartesianProduct 
+let uu___is_GS_Append (projectee : gather_strategy) : Prims.bool=
+  match projectee with | GS_Append -> true | uu___ -> false
+let uu___is_GS_CartesianProduct (projectee : gather_strategy) : Prims.bool=
+  match projectee with | GS_CartesianProduct -> true | uu___ -> false
+type gather_map =
+  {
+  gm_head: term_map ;
+  gm_members: term_map Prims.list ;
+  gm_as: gather_as ;
+  gm_strategy: gather_strategy ;
+  gm_allow_empty: Prims.bool }
+let __proj__Mkgather_map__item__gm_head (projectee : gather_map) : term_map=
+  match projectee with
+  | { gm_head; gm_members; gm_as; gm_strategy; gm_allow_empty;_} -> gm_head
+let __proj__Mkgather_map__item__gm_members (projectee : gather_map) :
+  term_map Prims.list=
+  match projectee with
+  | { gm_head; gm_members; gm_as; gm_strategy; gm_allow_empty;_} ->
+      gm_members
+let __proj__Mkgather_map__item__gm_as (projectee : gather_map) : gather_as=
+  match projectee with
+  | { gm_head; gm_members; gm_as; gm_strategy; gm_allow_empty;_} -> gm_as
+let __proj__Mkgather_map__item__gm_strategy (projectee : gather_map) :
+  gather_strategy=
+  match projectee with
+  | { gm_head; gm_members; gm_as; gm_strategy; gm_allow_empty;_} ->
+      gm_strategy
+let __proj__Mkgather_map__item__gm_allow_empty (projectee : gather_map) :
+  Prims.bool=
+  match projectee with
+  | { gm_head; gm_members; gm_as; gm_strategy; gm_allow_empty;_} ->
+      gm_allow_empty
+let decode_gather_as (l : RDF_Term.rdf_term Prims.list) : gather_as=
+  match l with
+  | (RDF_Term.T_IRI i)::uu___ ->
+      if i = rdf_List_str
+      then GA_List
+      else
+        if i = rdf_Bag_str
+        then GA_Bag
+        else
+          if i = rdf_Seq_str
+          then GA_Seq
+          else if i = rdf_Alt_str then GA_Alt else GA_Other i
+  | uu___ -> GA_List
+let decode_gather_strategy (l : RDF_Term.rdf_term Prims.list) :
+  gather_strategy=
+  match l with
+  | (RDF_Term.T_IRI i)::uu___ ->
+      if i = rml_cartesianProduct then GS_CartesianProduct else GS_Append
+  | uu___ -> GS_Append
+let decode_allow_empty (l : RDF_Term.rdf_term Prims.list) : Prims.bool=
+  match l with
+  | (RDF_Term.T_Literal lit)::uu___ -> lit.RDF_Term.lexical_form = "true"
+  | uu___ -> false
+let rec collect_gather_members (g : RDF_Graph.rdf_graph)
+  (head : RDF_Term.subject) (fuel : Prims.nat)
+  (acc : RDF_Term.subject Prims.list) : RDF_Term.subject Prims.list=
+  if fuel = Prims.int_zero
+  then FStar_List_Tot_Base.rev acc
+  else
+    (match RDF_Graph_Executable.find_objects g head rdf_first_iri with
+     | [] -> FStar_List_Tot_Base.rev acc
+     | m::uu___1 ->
+         let acc' =
+           match RDF_Graph.term_to_subject m with
+           | FStar_Pervasives_Native.Some ms -> ms :: acc
+           | FStar_Pervasives_Native.None -> acc in
+         (match RDF_Graph_Executable.find_objects g head rdf_rest_iri with
+          | r::uu___2 ->
+              (match RDF_Graph.term_to_subject r with
+               | FStar_Pervasives_Native.Some rs ->
+                   collect_gather_members g rs (fuel - Prims.int_one) acc'
+               | FStar_Pervasives_Native.None -> FStar_List_Tot_Base.rev acc')
+          | [] -> FStar_List_Tot_Base.rev acc'))
+let decode_gather_map (g : RDF_Graph.rdf_graph) (om_subj : RDF_Term.subject)
+  (fuel : Prims.nat) : gather_map=
+  let member_subjs =
+    match RDF_Graph_Executable.find_objects g om_subj rml_gather with
+    | h::uu___ ->
+        (match RDF_Graph.term_to_subject h with
+         | FStar_Pervasives_Native.Some hs ->
+             collect_gather_members g hs
+               ((RDF_Graph.graph_len g) + Prims.int_one) []
+         | FStar_Pervasives_Native.None -> [])
+    | [] -> [] in
+  {
+    gm_head = (decode_term_map_from_subject g om_subj fuel);
+    gm_members =
+      (FStar_List_Tot_Base.map
+         (fun ms -> decode_term_map_from_subject g ms fuel) member_subjs);
+    gm_as =
+      (decode_gather_as
+         (RDF_Graph_Executable.find_objects g om_subj rml_gatherAs));
+    gm_strategy =
+      (decode_gather_strategy
+         (RDF_Graph_Executable.find_objects g om_subj rml_strategy));
+    gm_allow_empty =
+      (decode_allow_empty
+         (RDF_Graph_Executable.find_objects g om_subj
+            rml_allowEmptyListAndContainer))
+  }
+let has_gather (g : RDF_Graph.rdf_graph) (s : RDF_Term.subject) : Prims.bool=
+  match RDF_Graph_Executable.find_objects g s rml_gather with
+  | [] -> false
+  | uu___ -> true
 type object_binding =
   | OB_TermMap of term_map 
   | OB_Join of ref_object_map 
+  | OB_Gather of gather_map 
 let uu___is_OB_TermMap (projectee : object_binding) : Prims.bool=
   match projectee with | OB_TermMap _0 -> true | uu___ -> false
 let __proj__OB_TermMap__item___0 (projectee : object_binding) : term_map=
@@ -524,6 +640,10 @@ let uu___is_OB_Join (projectee : object_binding) : Prims.bool=
   match projectee with | OB_Join _0 -> true | uu___ -> false
 let __proj__OB_Join__item___0 (projectee : object_binding) : ref_object_map=
   match projectee with | OB_Join _0 -> _0
+let uu___is_OB_Gather (projectee : object_binding) : Prims.bool=
+  match projectee with | OB_Gather _0 -> true | uu___ -> false
+let __proj__OB_Gather__item___0 (projectee : object_binding) : gather_map=
+  match projectee with | OB_Gather _0 -> _0
 type predicate_object_map =
   {
   pom_predicates: term_map Prims.list ;
@@ -541,13 +661,12 @@ let __proj__Mkpredicate_object_map__item__pom_graphs
   (projectee : predicate_object_map) : term_map Prims.list=
   match projectee with
   | { pom_predicates; pom_objects; pom_graphs;_} -> pom_graphs
-let decode_graphs (g : RDF_Graph_Executable.rdf_graph)
-  (s : RDF_Graph_Executable.subject) (fuel : Prims.nat) :
-  term_map Prims.list=
+let decode_graphs (g : RDF_Graph.rdf_graph) (s : RDF_Term.subject)
+  (fuel : Prims.nat) : term_map Prims.list=
   let via_map =
     FStar_List_Tot_Base.concatMap
       (fun t ->
-         match RDF_Graph_Executable.term_to_subject t with
+         match RDF_Graph.term_to_subject t with
          | FStar_Pervasives_Native.Some gs ->
              [decode_term_map_from_subject g gs fuel]
          | FStar_Pervasives_Native.None -> [])
@@ -556,13 +675,12 @@ let decode_graphs (g : RDF_Graph_Executable.rdf_graph)
     FStar_List_Tot_Base.map const_term_map
       (RDF_Graph_Executable.find_objects g s rml_graph) in
   FStar_List_Tot_Base.op_At via_map via_shortcut
-let decode_predicates (g : RDF_Graph_Executable.rdf_graph)
-  (s : RDF_Graph_Executable.subject) (fuel : Prims.nat) :
-  term_map Prims.list=
+let decode_predicates (g : RDF_Graph.rdf_graph) (s : RDF_Term.subject)
+  (fuel : Prims.nat) : term_map Prims.list=
   let via_map =
     FStar_List_Tot_Base.concatMap
       (fun t ->
-         match RDF_Graph_Executable.term_to_subject t with
+         match RDF_Graph.term_to_subject t with
          | FStar_Pervasives_Native.Some ps ->
              [decode_term_map_from_subject g ps fuel]
          | FStar_Pervasives_Native.None -> [])
@@ -571,49 +689,50 @@ let decode_predicates (g : RDF_Graph_Executable.rdf_graph)
     FStar_List_Tot_Base.map const_term_map
       (RDF_Graph_Executable.find_objects g s rml_predicate) in
   FStar_List_Tot_Base.op_At via_map via_shortcut
-let decode_object_bindings (g : RDF_Graph_Executable.rdf_graph)
-  (s : RDF_Graph_Executable.subject) (fuel : Prims.nat) :
-  object_binding Prims.list=
+let decode_object_bindings (g : RDF_Graph.rdf_graph) (s : RDF_Term.subject)
+  (fuel : Prims.nat) : object_binding Prims.list=
   let via_object_map =
     FStar_List_Tot_Base.concatMap
       (fun t ->
-         match RDF_Graph_Executable.term_to_subject t with
+         match RDF_Graph.term_to_subject t with
          | FStar_Pervasives_Native.None -> []
          | FStar_Pervasives_Native.Some om_subj ->
-             (match RDF_Graph_Executable.find_objects g om_subj
-                      rml_parentTriplesMap
-              with
-              | ptm::uu___ ->
-                  let parent_ref =
-                    match term_to_node_ref ptm with
-                    | FStar_Pervasives_Native.Some r -> r
-                    | FStar_Pervasives_Native.None -> "" in
-                  [OB_Join
-                     {
-                       rom_parent_triples_map = parent_ref;
-                       rom_joins = (decode_join_conditions g om_subj fuel)
-                     }]
-              | [] ->
-                  [OB_TermMap (decode_term_map_from_subject g om_subj fuel)]))
+             if has_gather g om_subj
+             then [OB_Gather (decode_gather_map g om_subj fuel)]
+             else
+               (match RDF_Graph_Executable.find_objects g om_subj
+                        rml_parentTriplesMap
+                with
+                | ptm::uu___1 ->
+                    let parent_ref =
+                      match term_to_node_ref ptm with
+                      | FStar_Pervasives_Native.Some r -> r
+                      | FStar_Pervasives_Native.None -> "" in
+                    [OB_Join
+                       {
+                         rom_parent_triples_map = parent_ref;
+                         rom_joins = (decode_join_conditions g om_subj fuel)
+                       }]
+                | [] ->
+                    [OB_TermMap (decode_term_map_from_subject g om_subj fuel)]))
       (RDF_Graph_Executable.find_objects g s rml_objectMap) in
   let via_object_shortcut =
     FStar_List_Tot_Base.map (fun t -> OB_TermMap (const_term_map t))
       (RDF_Graph_Executable.find_objects g s rml_object) in
   FStar_List_Tot_Base.op_At via_object_map via_object_shortcut
-let decode_predicate_object_map (g : RDF_Graph_Executable.rdf_graph)
-  (pom_subj : RDF_Graph_Executable.subject) (fuel : Prims.nat) :
-  predicate_object_map=
+let decode_predicate_object_map (g : RDF_Graph.rdf_graph)
+  (pom_subj : RDF_Term.subject) (fuel : Prims.nat) : predicate_object_map=
   {
     pom_predicates = (decode_predicates g pom_subj fuel);
     pom_objects = (decode_object_bindings g pom_subj fuel);
     pom_graphs = (decode_graphs g pom_subj fuel)
   }
-let decode_predicate_object_maps (g : RDF_Graph_Executable.rdf_graph)
-  (s : RDF_Graph_Executable.subject) (fuel : Prims.nat) :
+let decode_predicate_object_maps (g : RDF_Graph.rdf_graph)
+  (s : RDF_Term.subject) (fuel : Prims.nat) :
   predicate_object_map Prims.list=
   FStar_List_Tot_Base.concatMap
     (fun t ->
-       match RDF_Graph_Executable.term_to_subject t with
+       match RDF_Graph.term_to_subject t with
        | FStar_Pervasives_Native.Some pom_subj ->
            [decode_predicate_object_map g pom_subj fuel]
        | FStar_Pervasives_Native.None -> [])
@@ -621,20 +740,19 @@ let decode_predicate_object_maps (g : RDF_Graph_Executable.rdf_graph)
 type subject_map_t =
   {
   sm_term: term_map ;
-  sm_classes: RDF_Graph_Executable.wf_iri Prims.list ;
+  sm_classes: RDF_Term.wf_iri Prims.list ;
   sm_graphs: term_map Prims.list }
 let __proj__Mksubject_map_t__item__sm_term (projectee : subject_map_t) :
   term_map=
   match projectee with | { sm_term; sm_classes; sm_graphs;_} -> sm_term
 let __proj__Mksubject_map_t__item__sm_classes (projectee : subject_map_t) :
-  RDF_Graph_Executable.wf_iri Prims.list=
+  RDF_Term.wf_iri Prims.list=
   match projectee with | { sm_term; sm_classes; sm_graphs;_} -> sm_classes
 let __proj__Mksubject_map_t__item__sm_graphs (projectee : subject_map_t) :
   term_map Prims.list=
   match projectee with | { sm_term; sm_classes; sm_graphs;_} -> sm_graphs
-let decode_subject_map (g : RDF_Graph_Executable.rdf_graph)
-  (s : RDF_Graph_Executable.subject) (fuel : Prims.nat) :
-  subject_map_t FStar_Pervasives_Native.option=
+let decode_subject_map (g : RDF_Graph.rdf_graph) (s : RDF_Term.subject)
+  (fuel : Prims.nat) : subject_map_t FStar_Pervasives_Native.option=
   match RDF_Graph_Executable.find_objects g s rml_subjectMap with
   | [] ->
       (match RDF_Graph_Executable.find_objects g s rml_subject with
@@ -644,16 +762,13 @@ let decode_subject_map (g : RDF_Graph_Executable.rdf_graph)
              }
        | [] -> FStar_Pervasives_Native.None)
   | sm_term::[] ->
-      (match RDF_Graph_Executable.term_to_subject sm_term with
+      (match RDF_Graph.term_to_subject sm_term with
        | FStar_Pervasives_Native.None -> FStar_Pervasives_Native.None
        | FStar_Pervasives_Native.Some sm_subj ->
            let term = decode_term_map_from_subject g sm_subj fuel in
            let classes =
              FStar_List_Tot_Base.concatMap
-               (fun t ->
-                  match t with
-                  | RDF_Graph_Executable.T_IRI i -> [i]
-                  | uu___ -> [])
+               (fun t -> match t with | RDF_Term.T_IRI i -> [i] | uu___ -> [])
                (RDF_Graph_Executable.find_objects g sm_subj rml_class) in
            let graphs = decode_graphs g sm_subj fuel in
            FStar_Pervasives_Native.Some
@@ -695,36 +810,34 @@ type mapping_document = {
 let __proj__Mkmapping_document__item__md_triples_maps
   (projectee : mapping_document) : triples_map Prims.list=
   match projectee with | { md_triples_maps;_} -> md_triples_maps
-let decode_triples_map (g : RDF_Graph_Executable.rdf_graph)
-  (s : RDF_Graph_Executable.subject) (fuel : Prims.nat) : triples_map=
+let decode_triples_map (g : RDF_Graph.rdf_graph) (s : RDF_Term.subject)
+  (fuel : Prims.nat) : triples_map=
   {
     tm_id = (subject_to_node_ref s);
     tm_base_iri =
       (match RDF_Graph_Executable.find_objects g s rml_baseIRI with
-       | (RDF_Graph_Executable.T_IRI i)::uu___ ->
-           FStar_Pervasives_Native.Some i
+       | (RDF_Term.T_IRI i)::uu___ -> FStar_Pervasives_Native.Some i
        | uu___ -> FStar_Pervasives_Native.None);
     tm_logical_source = (decode_logical_source g s);
     tm_subject_map = (decode_subject_map g s fuel);
     tm_predicate_object_maps = (decode_predicate_object_maps g s fuel)
   }
-let is_triples_map_subject (g : RDF_Graph_Executable.rdf_graph)
-  (s : RDF_Graph_Executable.subject) : Prims.bool=
+let is_triples_map_subject (g : RDF_Graph.rdf_graph) (s : RDF_Term.subject) :
+  Prims.bool=
   FStar_List_Tot_Base.existsb
     (fun t ->
-       ((RDF_Graph_Executable.subject_eq t.RDF_Graph_Executable.s s) &&
-          (t.RDF_Graph_Executable.p = RDF_Graph_Executable.rdf_type))
+       ((RDF_Term.subject_eq t.RDF_Triple.s s) &&
+          (t.RDF_Triple.p = RDFS_Closure.rdf_type))
          &&
-         (RDF_Graph_Executable.rdf_term_eq t.RDF_Graph_Executable.o
-            (RDF_Graph_Executable.T_IRI rml_TriplesMap))) g
-let decode_mapping_document (g : RDF_Graph_Executable.rdf_graph) :
-  mapping_document=
+         (RDF_Term.rdf_term_eq t.RDF_Triple.o (RDF_Term.T_IRI rml_TriplesMap)))
+    g
+let decode_mapping_document (g : RDF_Graph.rdf_graph) : mapping_document=
   let subs = distinct_subjects g in
   let tm_subs = FStar_List_Tot_Base.filter (is_triples_map_subject g) subs in
   {
     md_triples_maps =
       (FStar_List_Tot_Base.map
          (fun s ->
-            decode_triples_map g s
-              ((RDF_Graph_Executable.graph_len g) + Prims.int_one)) tm_subs)
+            decode_triples_map g s ((RDF_Graph.graph_len g) + Prims.int_one))
+         tm_subs)
   }
